@prefix owl: <http://www.w3.org/2002/07/owl#> .
@prefix rdf: <http://www.w3.org/1999/02/22-rdf-syntax-ns#> .
@prefix rdfs: <http://www.w3.org/2000/01/rdf-schema#> .
@prefix saro: <http://w3id.org/saro#> .
@prefix badge: <https://w3id.org/openbadges/v2> .
@prefix skos: <http://www.w3.org/2004/02/skos/core#> .
@prefix ethon: <http://ethon.consensys.net/> .
@prefix qc: <http://w3id.org/qualichain#> .
@prefix schema: <http://schema.org/> .
@prefix xml: <http://www.w3.org/XML/1998/namespace> .
@prefix xsd: <http://www.w3.org/2001/XMLSchema#> .
@prefix cv: <http://rdfs.org/resume-rdf/cv.rdfs#> .



#To be reused

#saro:demand
#saro: sector
#saro: hasSkillGap
#saro: fillhasSkillGap 
#saro:JobPosting
#saro:Curriculum
#saro:TrainingResource (....courses)

#cv:CV
#cv:Person
#cv:aboutPerson
#cv:CV_Entry and all subclasses
#cv:Skill and all subclasses, and linked relationship to saro:Skill

qc:Person a owl:Class ;
    rdfs:label "User" ;
    rdfs:comment "A Person with accomplishments that can be verified on the blockchain." ;
    rdfs:subClassOf saro:User , cv:Person .

qc:Accomplishment a owl:Class ;
	rdfs:label "Accomplishment" ;
    rdfs:comment "Verifiable accomplishments of a Person." .
	
qc:hasResume a rdf:Property ;
	rdfs:label "hasResume" ;
    rdfs:comment "Links a person to a resume describing their accomplishments ." ;
    rdfs:domain qc:User ;
	owl:inverseOf cv:aboutPerson ;
    rdfs:range cv:cv .

qc:AwardingBody
    rdf:type owl:Class;
    rdfs:label "Awarding Body" ;
    rdfs:comment "The Educator or Trainer acting as an awarding body for an accomplishment" ;
    rdfs:subClassOf saro:EducatororTrainer ;
    schema:identifier qc:Profile .

qc:CertificationAuthority
    rdf:type owl:Class;
    rdfs:label "Certification Authority" ;
    rdfs:comment "An entity with the authority to certify the validity of accomplishments" .
    
qc:awardedBy a rdf:Property ;
    rdfs:label "awardedBy" ;
    rdfs:comment "This property is used to link an accomplishment to the body (educator, trainer) awarding it." ;
    rdfs:domain qc:Accomplishment ;
    rdfs:range qc:AwardingBody .

qc:certifiedBy a rdf:Property ;
    rdfs:label "certifiedBy" ;
    rdfs:comment "This property is used to link an accomplishment to the authority that certified its validity." ;
    rdfs:domain qc:Accomplishment ;
    rdfs:range qc:CertificationAuthority .

qc:refersToAccomplishment
	rdfs:label "refersToAccomplishment" ;
    rdfs:comment "An entry in a personal Resume refers to a known skill." ;
    rdfs:domain cv:CV_Entry ;
    rdfs:range qc:Accomplishment .

qc:verifiedBy a rdf:Property ;
    rdfs:label "verifiedby" ;
    rdfs:comment "To verify the authenticity of an individual identity, their accomplishments and the award of qualifications" ;
    rdfs:domain qc:Accomplishment ;
    rdfs:range qc:VerificationObject .
	
qc:VerificationObject
    rdf:type owl:Class ;
    rdfs:label "QualiChain Verification Object" ;
    rdfs:comment "an object containing QualiChain verification details." ;
    rdfs:subClassOf badge:VerificationObject .

qc:Profile 
    rdf:type owl:Class ;
    rdfs:label "QualiChain Badge Profile" ;
    rdfs:comment "Blockchain-backed Profile for OpenBadges" ;
    rdfs:subClassOf badge:Profile .

qc:blockchainProfileAccount a rdf:Property ;
    rdfs:label "blockchainprofileaccount" ;
    rdfs:comment "relating QualiChain Profiles to blockchain accounts" ;
    rdfs:domain qc:Profile ;
    rdfs:range ethon:ExternalAccount .

qc:blockchainContractAccount a rdf:Property ;
    rdfs:label "blockchaincontractaccount" ;
    rdfs:comment "relating QualiChain entities to blockchain contract accounts" ;
    rdfs:domain qc:VerificationObject ;
    rdfs:range ethon:ContractAccount .





