@prefix owl: <http://www.w3.org/2002/07/owl#> .
@prefix rdf: <http://www.w3.org/1999/02/22-rdf-syntax-ns#> .
@prefix rdfs: <http://www.w3.org/2000/01/rdf-schema#> .
@prefix saro: <http://w3id.org/saro#> .
@prefix badge: <https://w3id.org/openbadges/v2> .
@prefix skos: <http://www.w3.org/2004/02/skos/core#> .
@prefix ethon: <http://ethon.consensys.net/> .
@prefix qc: <http://w3id.org/qualichain#> .
@prefix schema: <http://schema.org/> .
@prefix xml: <http://www.w3.org/XML/1998/namespace> .
@prefix xsd: <http://www.w3.org/2001/XMLSchema#> .
@prefix cv: <http://rdfs.org/resume-rdf/cv.rdfs#> .


#To be reused

#saro:demand
#saro: sector
#saro: hasSkillGap
#saro: fillhasSkillGap 
#saro:JobPosting
#saro:Curriculum
#saro:TrainingResource (....courses)
#saro:Qualification (certificate)


qc:Person a owl:Class ;
    rdfs:label "Person" ;
    rdfs:comment "A Person with accomplishments that can be verified on the blockchain." ;
    rdfs:subClassOf saro:User , cv:Person .

qc:Accomplishment a owl:Class ;
    rdfs:label "Accomplishment" ;
    rdfs:comment "Verifiable accomplishments of a Person." .

qc:Qualification a owl:Class ;
    rdfs:label "Qualification" ;
    rdfs:comment "Extends the SARO Qualification class, which represents the official or formal certification of one or more acquired skills or competences." ;
    rdfs:subClassOf saro:Qualification, qc:Accomplishment .

qc:Experience a owl:Class ;
    rdfs:label "Experience" ;
    rdfs:comment "An accomplishment that does not consist of a qualification but of a veriafable work experience." ;
    rdfs:subClassOf qc:Accomplishment .


qc:AwardingBody
    rdf:type owl:Class;
    rdfs:label "Awarding Body" ;
    rdfs:comment "The Educator or Trainer acting as an awarding body for an accomplishment" ;
    rdfs:subClassOf saro:EducatororTrainer ;
    schema:identifier qc:Profile .

qc:hasAccomplishment a rdf:Property ;
    rdfs:label "has Accomplishment" ;
    rdfs:comment "This property is used to link a person to their verifiable accomplishments (experiences, skills, qualifications, awards)." ;
    rdfs:domain qc:Person ;
    rdfs:range qc:Accomplishment .


qc:CertificationAuthority
    rdf:type owl:Class;
    rdfs:label "Certification Authority" ;
    rdfs:comment "An entity with the authority to certify the validity of accomplishments" .
  
qc:awardedBy a rdf:Property ;
    rdfs:label "awardedBy" ;
    rdfs:comment "This property is used to link an accomplishment to the body (educator, trainer) awarding it." ;
    rdfs:domain qc:Accomplishment ;
    rdfs:range qc:AwardingBody .

qc:certifiedBy a rdf:Property ;
    rdfs:label "certifiedBy" ;
    rdfs:comment "This property is used to link an accomplishment to the authority that certified its validity." ;
    rdfs:domain qc:Accomplishment ;
    rdfs:range qc:CertificationAuthority .

qc:verifiedBy a rdf:Property ;
    rdfs:label "verifiedby" ;
    rdfs:comment "To verify the authenticity of an individual identity, their accomplishments and the award of qualifications" ;
    rdfs:domain qc:Accomplishment ;
    rdfs:range qc:VerificationObject .
	
qc:VerificationObject
    rdf:type owl:Class ;
    rdfs:label "Verification Object" ;
    rdfs:comment "An object containing Verification details." ;
    rdfs:subClassOf badge:VerificationObject .

qc:Profile 
    rdf:type owl:Class ;
    rdfs:label "Profile" ;
    rdfs:comment "Blockchain-backed Profile for OpenBadges" ;
    rdfs:subClassOf badge:Profile .

qc:hasProfile  a rdf:Property ;
    rdfs:label "has Profile" ;
    rdfs:comment "Links entities (as recipients of Badges) or organisations (as Badge Issuer) to an OpenBadges Profile" ;
    rdfs:domain qc:User , qc:Awarding Body ;
    rdfs:range qc:Profile .
	
qc:blockchainProfileAccount a rdf:Property ;
    rdfs:label "blockchain Profile Account" ;
    rdfs:comment "Links profiles to blockchain accounts" ;
    rdfs:domain qc:Profile ;
    rdfs:range ethon:ExternalAccount .

qc:blockchainContractAccount a rdf:Property ;
    rdfs:label "blockchain Contract Account" ;
    rdfs:comment "Linkes entities to blockchain contract accounts" ;
    rdfs:domain qc:VerificationObject ;
    rdfs:range ethon:ContractAccount .

#Resume descriptive elements. Note: elements from a Resume should always point to other elements described here or in other vocabularies and never the other way around. For example, it does not make sense to link an actual Work Experience to a CV owned by someone describing it. Instead, the CV description can point to the work experience, in that direction.
#cv:CV
#cv:Person
#cv:aboutPerson
#cv:CV_Entry and all subclasses
#cv:Skill and all subclasses, and linked relationship to saro:Skill

qc:hasResume a rdf:Property ;
	rdfs:label "has Resume" ;
    rdfs:comment "Links a person to a resume describing their accomplishments ." ;
    rdfs:domain qc:Person ;
	owl:inverseOf cv:aboutPerson ;
    rdfs:range cv:CV .

qc:refersToAccomplishment a rdf:Property ;
  rdfs:label "refers To Accomplishment" ;
  rdfs:comment "Links a Resume to verifiable accomplishments ." ;
  rdfs:domain cv:CV_Entry ;
  rdfs:range qc:Accomplishment .

qc:refersToExperience  a rdf:Property ;
  rdfs:subPropertyOf qc:refersToAccomplishment ;
  rdfs:label "refers to Experience" ;
  rdfs:comment "Links a CV Work History entry to a verifiable work experience." ;
  rdfs:domain cv:WorkHistory ;
  rdfs:range qc:Experience .

qc:refersToQualification  a rdf:Property ;
  rdfs:subPropertyOf qc:refersToAccomplishment ;
  rdfs:label "refers to Qualification" ;
  rdfs:comment "Links a CV entry (Course, Education or Skill) to a verifiable qualification." ;
  rdfs:domain cv:Course , cv:Education, cv:Skill ;
  rdfs:range qc:Qualification .

#Link Profile to CV vocab 
#qc:Profile 
    #rdf:type owl:Class ;
    #rdfs:label "Badge Profile" ;
    #rdfs:comment "Blockchain-backed Profile for OpenBadges" ;
    #rdfs:subClassOf badge:Profile .

#cv:course coveredBy saro:Curriculum 


